\documentclass[10pt,a4paper]{article}
\usepackage[landscape]{geometry}
\usepackage{fullpage}
\usepackage{breqn}
\begin{document}
\footnotesize
\begin{dmath}
% Equation 1
{g}=\phi+\phi\, {\lambda}\, \left({Z_D}-1\right)
\end{dmath}
\begin{dmath}
% Equation 2
{g}\, {Z_D}=\phi\, {Z_D}+{V_D}
\end{dmath}
\begin{dmath}
% Equation 3
{V_D}={Z_D}\, {\overline{\zeta}}\, {\zeta}\, \left(\frac{{g}\, {N_D}}{{K_D}}\right)^{\eta}
\end{dmath}
\begin{dmath}
% Equation 4
{J}=\left(-{M}\right)+\phi\, {\Lambda}\, \left({\lambda}\, {H}+{J}\, \left(1-{\lambda}\right)\right)
\end{dmath}
\begin{dmath}
% Equation 5
{H}={\Pi}+\phi\, {\Lambda}\, {H}
\end{dmath}
\begin{dmath}
% Equation 6
{\Pi}=\frac{1}{\vartheta}\, \frac{1}{{\mathcal{M}}}\, {Y^W_D}
\end{dmath}
\begin{dmath}
% Equation 7
{Z_D}\, {\zeta}\, {\overline{\zeta}}\, {J}\, {\Lambda}\, \frac{1}{\left(\frac{{K_D}}{{g}}\right)^{\eta}}\, \frac{1}{{N_D}^{1-\eta}}\, \frac{1}{{\Delta^N}}=1+log\left({\left.       f^{\prime}\left( \cdot \right)   \right|}\right)\, \frac{{g}\, {N_D}}{{N_D}}+log\left({\left.       f\left( \cdot \right)            \right|}\right)-{\Lambda}\, log\left({\left.       f^{\prime}\left( \cdot \right)   \right|}\right)\, \left(\frac{{g}\, {N_D}}{{N_D}}\right)^{2}
\end{dmath}
\begin{dmath}
% Equation 8
{\Lambda}\, \phi\, {\rho_\lambda}\, {\bar{\lambda}}\, \left({H}-{J}\right)\, \frac{1}{{\Delta^M}}={M}^{1-{\rho_\lambda}}
\end{dmath}
\begin{dmath}
% Equation 9
{\lambda}={\bar{\lambda}}\, {M}^{{\rho_\lambda}}
\end{dmath}
\begin{dmath}
% Equation 10
{Y_D}={Y^W_D}
\end{dmath}
\begin{dmath}
% Equation 11
{Y^W_D}=\left(\frac{{K_D}}{{g}}\right)^{\alpha}\, {L}^{1-\alpha}
\end{dmath}
\begin{dmath}
% Equation 12
{Y_D}={C_D}+\left(1+log\left({\left.       g\left( \cdot \right)            \right|}\right)\right)\, {I_D}+{N_D}\, \left(1+log\left({\left.       f\left( \cdot \right)            \right|}\right)\right)+\left({Z_D}-1\right)\, {M}
\end{dmath}
\begin{dmath}
% Equation 13
{\Lambda}=\frac{\beta\, {U_{CD}}}{{U_{CD}}}\, {g}^{\left(-\rho\right)}
\end{dmath}
\begin{dmath}
% Equation 14
{U_{CD}}=\left({C_D}-{\Gamma_D}\, \frac{\chi}{1+\epsilon}\, {L}^{1+\epsilon}\right)^{\left(-\rho\right)}-{{\mu}_{D}}\, \gamma\, \left(\frac{{\Gamma_D}}{{g}\, {C_D}}\right)^{1-\gamma}
\end{dmath}
\begin{dmath}
% Equation 15
{{\mu}_{D}}=\beta\, \left(1-\gamma\right)\, {g}^{\left(-\rho\right)}\, {{\mu}_{D}}\, \left(\frac{{g}\, {C_D}}{{\Gamma_D}}\right)^{\gamma}+{L}^{1+\epsilon}\, \frac{\chi}{1+\epsilon}\, \left({C_D}-{\Gamma_D}\, \frac{\chi}{1+\epsilon}\, {L}^{1+\epsilon}\right)^{\left(-\rho\right)}
\end{dmath}
\begin{dmath}
% Equation 16
\left({C_D}-{\Gamma_D}\, \frac{\chi}{1+\epsilon}\, {L}^{1+\epsilon}\right)^{\left(-\rho\right)}\, {\Gamma_D}\, \chi\, {L}^{\epsilon}\, \frac{1}{{U_{CD}}}=\left(1-\alpha\right)\, \frac{1}{{\mathcal{M}}}\, \frac{\vartheta-1}{\vartheta}\, \frac{{Y_D}}{{L}}
\end{dmath}
\begin{dmath}
% Equation 17
{\Gamma_D}={C_D}^{\gamma}\, \left(\frac{{\Gamma_D}}{{g}}\right)^{1-\gamma}
\end{dmath}
\begin{dmath}
% Equation 18
{K_D}={I_D}+\frac{{K_D}}{{g}}\, \left(1-\delta\right)
\end{dmath}
\begin{dmath}
% Equation 19
{Q}=1+log\left({\left.       g\left( \cdot \right)            \right|}\right)+\frac{{g}\, {I_D}}{{I_D}}\, log\left({\left.       g^{\prime}\left( \cdot \right)   \right|}\right)-log\left({\left.       g^{\prime}\left( \cdot \right)   \right|}\right)\, {\Lambda}\, \left(\frac{{g}\, {I_D}}{{I_D}}\right)^{2}
\end{dmath}
\begin{dmath}
% Equation 20
{Q}={\Lambda}\, \left(\frac{\alpha\, {Y^W_D}\, {g}\, \left(\vartheta-1\right)}{\vartheta\, {K_D}\, {\mathcal{M}}}+\left(1-\delta\right)\, {Q}\right)
\end{dmath}
\begin{dmath}
% Equation 21
log\left({\zeta}\right)=log\left({\zeta}\right)\, {{\rho}_{\zeta}}+{{\sigma}_{\zeta}}\, {\epsilon}^{\chi}
\end{dmath}
\begin{dmath}
% Equation 22
{\mathcal{S}_{D}}={H}+{K_D}\, {Q}+{J}\, \left({Z_D}+{V_D}-1\right)+{X_D}
\end{dmath}
\begin{dmath}
% Equation 23
{X_D}={g}\, {\Lambda}\, \left({X_D}+{V_D}\, {J}\right)
\end{dmath}
\begin{dmath}
% Equation 24
{\mathcal{R}_{D}}={N_D}
\end{dmath}
\begin{dmath}
% Equation 25
log\left({\Delta^N}\right)=log\left({\Delta^N}\right)\, {\rho}_n-{\sigma}_n\, {\epsilon}^n
\end{dmath}
\begin{dmath}
% Equation 26
log\left({\Delta^M}\right)=log\left({\Delta^N}\right)\, \alpha_N
\end{dmath}
\begin{dmath}
% Equation 27
{\left.       f\left( \cdot \right)            \right|}=exp\left(\frac{{\psi_N}}{2}\, \left(\frac{{g}\, {N_D}}{{N_D}}-{g^{SS}}\right)^{2}\right)
\end{dmath}
\begin{dmath}
% Equation 28
{\left.       f^{\prime}\left( \cdot \right)   \right|}=exp\left({\psi_N}\, \left(\frac{{g}\, {N_D}}{{N_D}}-{g^{SS}}\right)\right)
\end{dmath}
\begin{dmath}
% Equation 29
{\left.       g\left( \cdot \right)            \right|}=exp\left(\frac{{\psi_I}}{2}\, \left(\frac{{g}\, {I_D}}{{I_D}}-{g^{SS}}\right)^{2}\right)
\end{dmath}
\begin{dmath}
% Equation 30
{\left.       g^{\prime}\left( \cdot \right)   \right|}=exp\left({\psi_I}\, \left(\frac{{g}\, {I_D}}{{I_D}}-{g^{SS}}\right)\right)
\end{dmath}
\begin{dmath}
% Equation 31
{\pi}^{1-{\omega}}={\theta}+\left(1-{\theta}\right)\, {\pi^*}^{1-{\omega}}
\end{dmath}
\begin{dmath}
% Equation 32
{\pi^*}={\pi}\, \frac{{\omega}}{{\omega}-1}\, \frac{{x_{1D}}}{{x_{2D}}}
\end{dmath}
\begin{dmath}
% Equation 33
{x_{1D}}={Y_D}\, \frac{1}{{\mathcal{M}}}\, {U_{CD}}+{x_{1D}}\, \beta\, {\theta}\, {g}^{1-\rho}\, {\pi}^{{\omega}}
\end{dmath}
\begin{dmath}
% Equation 34
{x_{2D}}={Y_D}\, {U_{CD}}+{x_{2D}}\, \beta\, {\theta}\, {g}^{1-\rho}\, {\pi}^{{\omega}-1}
\end{dmath}
\begin{dmath}
% Equation 35
1=\frac{{\Lambda}\, {R}}{{\pi}}
\end{dmath}
\begin{dmath}
% Equation 36
\frac{{R}}{\left(\beta\, {g^{SS}}^{\left(-\rho\right)}\right)^{\left(-1\right)}}={\pi}^{{{\gamma}_{\pi}}}\, \left(\frac{\frac{1}{{\mathcal{M}}}}{\frac{1}{{\mkup^{SS}}}}\right)^{{{\gamma}_{y}}}
\end{dmath}
\end{document}
